Current draft

src/SmallSteps.v
@@ -32,12 +32,44 @@ Module C.
   Inductive t (E : Effect.t) (A : Type) : Type :=
   | Ret : A -> t E A
   | Call : forall c, (Effect.answer E c -> t E A) -> t E A
-  | Join : forall {B C : Type}, t E B -> t E C -> (B * C -> t E A) -> t E A
-  | Choose : forall {B : Type}, t E B -> t E B -> (B -> t E A) -> t E A.
+  | Join : forall (B C : Type), t E B -> t E C -> (B * C -> t E A) -> t E A
+  | Choose : forall (B : Type), t E B -> t E B -> (B -> t E A) -> t E A.
   Arguments Ret {E A} _.
   Arguments Call {E A} _ _.
   Arguments Join {E A B C} _ _ _.
   Arguments Choose {E A B} _ _ _.
+
+  Module StrictC.
+    Inductive t (E : Effect.t) (A : Type) : Type :=
+    | Call : forall c, (Effect.answer E c -> t E A) -> t E A
+    | CallRet : forall c, (Effect.answer E c -> A) -> t E A
+    | Let : forall (B : Type)
+    | Join : forall (B C : Type), t E B -> t E C -> (B * C -> t E A) -> t E A
+    | Choose : forall (B : Type), t E B -> t E B -> (B -> t E A) -> t E A.
+    Arguments Call {E A} _ _.
+    Arguments CallRet {E A} _ _.
+    Arguments Join {E A B C} _ _ _.
+    Arguments Choose {E A B} _ _ _.
+
+    Module Step.
+      Inductive t {E : Effect.t} {A : Type} (e : Event.t E)
+        : StrictC.t E A -> StrictC.t E A -> Type :=
+      | Call : forall h,
+        t e (C.Call (Event.c e) h) (h (Event.a e))
+      | JoinLeft : forall B C (x : C.t E B) (y : C.t E C) k x',
+        t e (A := B) x x' ->
+        t e (C.Join x y k) (join x' y k)
+      | JoinRight : forall B C (x : C.t E B) (y : C.t E C) k y',
+        t e (A := C) y y' ->
+        t e (C.Join x y k) (join x y' k)
+      | ChooseLeft : forall x1 x2 k x1',
+        t e x1 x1' ->
+        t e (C.Choose x1 x2 k) (bind x1' k)
+      | ChooseRight : forall x1 x2 k x2',
+        t e x2 x2' ->
+        t e (C.Choose x1 x2 k) (bind x2' k).
+    End Step.
+  End StrictC.
 
   Fixpoint bind {E A B} (x : t E A) (f : A -> t E B) : t E B :=
     match x with
@@ -211,6 +243,23 @@ Module Choose.
             bind (k_y y) (fun y =>
             Ret (x, y))))
       end.
+
+    Fixpoint equiv_left {E} : forall {A B C} e (x x' : Choose.t E A) (y : Choose.t E B)
+      (k : A * B -> Choose.t E C) (m_xy : t x y) (m_x'y : t x' y),
+      Step.t e x x' -> Step.t e (bind (join m_xy) k) (bind (join m_x'y) k).
+      (*intros.
+      destruct X.
+      - destruct y.
+        + assert (m_xy = CallRet (Event.c e) h b).
+          inversion m_xy.
+        inversion m_xy.
+      destruct m_xy.*)
+    Admitted.
+
+    (*Fixpoint equiv_right {E} : forall {A B C} e (x : Choose.t E A) (y y' : Choose.t E B)
+      (k : A * B -> Choose.t E C) (m_xy : t x y) (m_xy' : t x y'),
+      Step.t e y y' -> Step.t e (join m_xy) (join m_xy').
+    Admitted.*)
   End Mix.
 
   Fixpoint compile {E A} (x : C.t E A) : t E A :=
@@ -223,4 +272,27 @@ Module Choose.
     | C.Choose _ x y k =>
       Choose (compile x) (compile y) (fun xy => compile (k xy))
     end.
+
+  Lemma equiv_join_bind {E A B C} (x : C.t E A) (y : C.t E B) (k : A * B -> C.t E C)
+    compile (C.join x y) k -> bind (compile .
+
+  Fixpoint equiv {E} : forall {A} (e : Event.t E) (x x' : C.t E A),
+    C.Step.t e x x' -> Step.t e (compile x) (compile x').
+    intros A e x x' H.
+    destruct H.
+    - simpl.
+      apply (Step.Call e (fun a => compile (h a))).
+    - simpl.
+      Check Mix.equiv_left e (compile x) (compile x') (compile y)
+        (fun xy => compile (k xy))
+        (Mix.make (compile x) (compile y)) (Mix.make (compile x') (compile y))
+        (equiv E B e x x' H). _ _ _ _ H.
+      destruct H.
+      + destruct (compile y).
+        * simpl.
+          Check Step.Call e (fun a =>
+      bind (bind (compile (h a)) (fun x => Ret (x, c)))
+        (fun xy => compile (k xy)).
+      
+  Defined.
 End Choose.
